execution/tests/EIP20TokenTests.v
@@ -14,7 +14,7 @@ From ConCert Require Import EIP20Token.
 Require Import Extras.
 
 From ConCert.Execution.QCTests Require Import 
-	ChainGens TestUtils ChainPrinters SerializablePrinters EIP20TokenPrinters EIP20TokenGens.
+	ChainGens TestUtils ChainPrinters SerializablePrinters EIP20TokenPrinters EIP20TokenGens TraceGens.
 
 (* For monad notations *)
 Require Export ExtLib.Structures.Monads.
@@ -31,3 +31,141 @@ Import BoundedN.Stdpp.
 Import LocalBlockchain.
 Import ListNotations.
 Close Scope address_scope.
+
+
+(* -------------------------- Tests of the EIP20 Token Implementation -------------------------- *)
+
+Definition token_setup := EIP20Token.build_setup creator 100.
+Definition deploy_eip20token : @ActionBody Base := create_deployment 0 EIP20Token.contract token_setup.
+
+Let contract_base_addr := BoundedN.of_Z_const AddrSize 128%Z.
+
+Definition chain_with_token_deployed :=  
+  unpack_option (my_add_block lc_initial 
+  [
+    build_act creator (act_transfer person_1 10);
+    build_act creator (act_transfer person_2 10);
+    build_act creator (act_transfer person_3 10);
+    build_act creator deploy_eip20token
+  ]).
+
+Definition gEIP20TokenChainTraceList lc length := 
+  gLocalChainTraceList_fix lc (fun lc _ => 
+    gEIP20TokenAction lc contract_base_addr) length.
+
+
+Definition token_reachableFrom (lc : LocalChain) pf : Checker := 
+  @reachableFrom AddrSize lc gEIP20TokenChainTraceList pf.
+
+Definition token_reachableFrom_implies_reachable (lc : LocalChain) pf1 pf2 : Checker := 
+  reachableFrom_implies_reachable lc gEIP20TokenChainTraceList pf1 pf2.
+
+Compute (show (map fst (FMap.elements (lc_contracts chain_with_token_deployed)))).
+Compute (show (lc_token_contracts_states_deserialized chain_with_token_deployed)).
+Compute (show (lc_account_balances chain_with_token_deployed)).
+(* Sample (gEIP20TokenChainTraceList chain_with_token_deployed 10). *)
+Open Scope string_scope.
+Definition debug_gEIP20Checker lc (act : option Action) :=
+  let print_valid_actions := match act with
+                            | Some act => "valid actions: " ++ show (validate_actions [act]) ++ sep ++ nl
+                            | None => ""
+                            end in
+  whenFail 
+    ("lc balances: " ++ show (lc_account_balances lc) ++ sep ++ nl
+    ++ print_valid_actions
+    ++ "token state: " ++ show (lc_token_contracts_states_deserialized lc) ++ sep ++ nl 
+    ).
+
+
+(* QuickChick (forAll 
+  (gEIP20TokenAction chain_with_token_deployed contract_base_addr) 
+  (fun act_opt => isSomeCheck act_opt (fun act => 
+    (isSomeCheck (my_add_block chain_with_token_deployed [act]) (fun _ => checker true))
+  ))). *)
+(* coqtop-stdout:+++ Passed 10000 tests (0 discards) *)
+
+(* Sample (gEIP20TokenAction chain_with_token_deployed contract_base_addr). *)
+Sample (gEIP20TokenChainTraceList chain_with_token_deployed 10).
+(* QuickChick (forAll 
+  (gEIP20TokenAction chain_with_token_deployed contract_base_addr) 
+  (fun act_opt => isSomeCheck act_opt (fun act => 
+    (debug_gEIP20Checker chain_with_token_deployed (Some act))  
+      ((checker o isSome) (my_add_block chain_with_token_deployed [act]))))). *)
+(* coqtop-stdout:+++ Passed 10000 tests (0 discards) *)
+
+Definition last_state trace := List.last (map next_lc_of_lcstep trace) chain_with_token_deployed.
+
+
+(* Generate a trace, and then execute an action on the last state of the trace. Check that this always succeeds *)
+(* QuickChick (forAll2 
+  (gEIP20TokenChainTraceList chain_with_token_deployed 5) 
+  (fun trace => 
+    gEIP20TokenAction (last_state trace) 
+                      contract_base_addr)
+  (fun trace act_opt => isSomeCheck act_opt (fun act => 
+    (debug_gEIP20Checker (last_state trace) (Some act))  
+      ((checker o isSome) (my_add_block (last_state trace) [act]))))). *)
+
+
+Open Scope nat_scope.
+(* One key property: the sum of the balances is always equal to the initial supply *)
+Definition sum_balances_eq_init_supply_P maxLength := 
+  forAllTraces maxLength chain_with_token_deployed gEIP20TokenChainTraceList
+    (fun (lc : LocalChain) =>
+      debug_gEIP20Checker lc None
+      (checker match FMap.find contract_base_addr (lc_token_contracts_states_deserialized lc) with
+      | Some state => 
+        let balances_list := (map snd o FMap.elements) state.(balances) in
+        let balances_sum : nat := fold_left plus balances_list 0 in
+        balances_sum =? state.(total_supply)
+      | None => false
+      end)).
+
+(* QuickChick (sum_balances_eq_init_supply_P 7). *)
+(* coqtop-stdout:+++ Passed 10000 tests (0 discards) *)
+
+(* INVALID PROPERTY: accounts may allow multiple other accounts to transfer tokens, but the actual transfer ensures that
+   no more tokens are sent than the balance of the sender. *)
+Definition sum_allowances_le_init_supply_P maxLength :=
+  forAllTraces maxLength chain_with_token_deployed gEIP20TokenChainTraceList
+    (fun (lc : LocalChain) =>
+      debug_gEIP20Checker lc None
+      (checker match FMap.find contract_base_addr (lc_token_contracts_states_deserialized lc) with
+      | Some state => 
+        let allowances := map_values_FMap 
+          (fun allowance_map => fold_left plus ((map snd o FMap.elements) allowance_map) 0)
+          state.(allowances) in
+        let allowances_list := (map snd o FMap.elements) allowances in
+        let allowances_sum := fold_left plus allowances_list 0 in 
+        allowances_sum <=? state.(total_supply)
+      | None => false
+      end)).
+    
+(* QuickChick (sum_allowances_le_init_supply_P 5). *)
+
+Definition person_has_tokens person (n : nat) := 
+  fun lc =>
+    match FMap.find contract_base_addr (lc_token_contracts_states_deserialized lc) with
+    | Some state => n =? (FMap_find_ person state.(balances) 0)  
+    | None => false
+    end.
+
+Notation "lc '~~>' pf" :=
+  (token_reachableFrom lc pf)
+  (at level 45, no associativity).
+
+
+
+(* QuickChick (chain_with_token_deployed ~~> person_has_tokens person_3 12). *)
+(* QuickChick (chain_with_token_deployed ~~> person_has_tokens creator 0). *)
+
+QuickChick (token_reachableFrom_implies_reachable 
+  chain_with_token_deployed
+  (person_has_tokens creator 10)
+  (person_has_tokens creator 0)        
+).
+
+(* Notation "lc '~~>' pf1 '~~>' pf2" :=
+  (token_reachableFrom_implies_reachable lc pf1 pf2)   
+  (at level 99).
+QuickChick (chain_with_token_deployed ~~> person_has_tokens creator 0 ~~> person_has_tokens creator 10 ). *)
